lakefile.lean
@@ -5,7 +5,7 @@ package "connect4" where
   version := v!"0.1.0"
 
 require mathlib from git
-  "https://github.com/leanprover-community/mathlib4.git" @ "main"
+  "https://github.com/leanprover-community/mathlib4.git" @ "master"
 
 lean_lib «Connect4» where
   roots := #[`Connect4]
